push changes

src/Std/Data/DTreeMap/Raw/Basic.lean
@@ -736,6 +736,19 @@ instance : Inter (Raw α β cmp) := ⟨inter⟩
 def eraseMany {ρ} [ForIn Id ρ α] (t : Raw α β cmp) (l : ρ) : Raw α β cmp :=
   letI : Ord α := ⟨cmp⟩; ⟨t.inner.eraseMany! l⟩
 
+@[inline, inherit_doc DTreeMap.eraseMany]
+def eraseManyEntries {ρ} [ForIn Id ρ ((a : α) × β a)] (t : Raw α β cmp) (l : ρ) : Raw α β cmp :=
+  letI : Ord α := ⟨cmp⟩; ⟨t.inner.eraseManyEntries! l⟩
+
+/--
+Computes the diffrence of the given tree maps.
+This function always iteraters through the smaller map.
+-/
+def diff (t₁ t₂ : Raw α β cmp) : Raw α β cmp :=
+  letI : Ord α := ⟨cmp⟩; ⟨t₁.inner.diff! t₂.inner⟩
+
+instance : SDiff (Raw α β cmp) := ⟨diff⟩
+
 namespace Const
 
 variable {β : Type v}
