src/Std/Data/DTreeMap/Raw/WF.lean
@@ -89,6 +89,10 @@ theorem eraseMany [TransCmp cmp] {ρ} [ForIn Id ρ α] {l : ρ} {t : Raw α β c
     (h : t.WF) : WF (t.eraseMany l) :=
   ⟨h.out.eraseMany!⟩
 
+theorem eraseManyEntries [TransCmp cmp] {ρ} [ForIn Id ρ ((a : α) × β a)] {l : ρ} {t : Raw α β cmp}
+    (h : t.WF) : WF (t.eraseManyEntries l) :=
+  ⟨h.out.eraseManyEntries!⟩
+
 theorem insertMany [TransCmp cmp] {ρ} [ForIn Id ρ ((a : α) × β a)] {l : ρ} {t : Raw α β cmp}
     (h : t.WF) : WF (t.insertMany l) :=
   ⟨h.out.insertMany!⟩
@@ -164,5 +168,9 @@ theorem union [TransCmp cmp] {t₁ t₂ : Raw α β cmp} (h₁ : t₁.WF) (h₂ 
 theorem inter [TransCmp cmp] {t₁ t₂ : Raw α β cmp} (h₁ : t₁.WF) :
     (t₁ ∩ t₂).WF :=
   ⟨Impl.WF.inter! h₁.out⟩
+
+theorem diff [TransCmp cmp] {t₁ t₂ : Raw α β cmp} (h₁ : t₁.WF) :
+    (t₁ \ t₂).WF :=
+  ⟨Impl.WF.diff! h₁.out⟩
 
 end Std.DTreeMap.Raw.WF.Const
